generator progress

PivotBetree/BucketGenerator.i.dfy
@@ -23,22 +23,160 @@ module BucketGenerator {
         // Bucket that the generator represents
         ghost remains: Bucket
       )
+    | MergeGenerator(
+        // "Internals":
+        top: Generator,
+        bot: Generator,
+        next: IteratorOutput,
+
+        // Bucket that the generator represents
+        ghost remains: Bucket
+      )
 
   protected predicate WF(g: Generator)
   {
-    && WFIter(g.bucket, g.it)
-    && (g.it.next.Done? ==> g.remains == map[])
-    && (g.it.next.Next? ==> Keyspace.minimumOpt(g.remains.Keys) == Some(g.it.next.key))
+    && (g.BasicGenerator? ==> (
+      && WFIter(g.bucket, g.it)
+      && (g.it.next.Done? ==> g.remains == map[])
+      && (g.it.next.Next? ==> Keyspace.minimumOpt(g.remains.Keys) == Some(g.it.next.key))
+      && (g.it.next.Next? ==> g.remains == 
+            map k | k in g.bucket && Keyspace.lte(g.it.next.key, k) :: g.bucket[k])
+    ))
+    && (g.MergeGenerator? ==> (
+      && WF(g.top)
+      && WF(g.bot)
+      && (g.next.Next? ==> (
+        && (forall k | k in g.top.remains :: Keyspace.lt(g.next.key, k))
+        && (forall k | k in g.bot.remains :: Keyspace.lt(g.next.key, k))
+        && g.remains == Lump(g.top.remains, g.bot.remains)[g.next.key := g.next.msg]
+      ))
+      && (g.next.Done? ==> (
+        && g.top.remains == map[]
+        && g.bot.remains == map[]
+        && g.remains == map[]
+      ))
+    ))
   }
 
   // Generator operations:
+
+  lemma lemmaMergeGenTop(g: Generator)
+  requires WF(g)
+  requires g.MergeGenerator?
+  ensures g.next.Next? ==> Keyspace.minimumOpt(g.remains.Keys) == Some(g.next.key);
+  {
+    reveal_Lump();
+    if g.next.Next? {
+      assert g.next.key in g.remains.Keys;
+      //assert forall k | k in g.remains.Keys :: Keyspace.lte(g.next.key, k);
+      //assert Keyspace.minimumOpt(g.remains.Keys) == Some(g.next.key);
+    }
+  }
 
   function {:opaque} GenTop(g: Generator) : (next : IteratorOutput)
   requires WF(g)
   ensures next.Done? ==> g.remains == map[]
   ensures next.Next? ==> Keyspace.minimumOpt(g.remains.Keys) == Some(next.key)
   {
-    g.it.next
+    match g {
+      case BasicGenerator(bucket, it, remains) => (
+        //assert g.it.next.Next? ==> Keyspace.minimumOpt(g.remains.Keys) == Some(g.it.next.key);
+        g.it.next
+      )
+      case MergeGenerator(top, bot, next, remains) => (
+        lemmaMergeGenTop(g);
+        g.next
+      )
+    }
+  }
+
+  function BasicGenPop(g: Generator) : (g' : Generator)
+  requires WF(g)
+  requires GenTop(g).Next?
+  requires g.BasicGenerator?
+  {
+    var remains := MapRemove1(g.remains, GenTop(g).key);
+
+    BasicGenerator(
+      g.bucket,
+      IterInc(g.bucket, g.it),
+      remains)
+  }
+
+  lemma lemmaBasicGenPop(g: Generator)
+  requires BasicGenPop.requires(g)
+  ensures WF(BasicGenPop(g))
+  {
+    var g' := BasicGenPop(g);
+    if g'.it.next.Done? {
+      forall k | k in g'.remains
+      ensures false
+      {
+        noKeyBetweenIterAndIterInc(g.bucket, g.it, k);
+      }
+    }
+    if g'.it.next.Next? {
+      IterIncKeyGreater(g.bucket, g.it);
+      //assert Keyspace.lte(g.it.next.key, g'.it.next.key);
+      //assert g'.it.next.key in g.remains.Keys;
+      //assert g'.it.next.key != GenTop(g).key;
+      assert g'.it.next.key in g'.remains.Keys;
+      forall k | k in g'.remains.Keys
+      ensures Keyspace.lte(g'.it.next.key, k)
+      {
+        noKeyBetweenIterAndIterInc(g.bucket, g.it, k);
+      }
+    }
+  }
+
+  function MergeGenPop(g: Generator) : (g' : Generator)
+  requires WF(g)
+  requires GenTop(g).Next?
+  requires g.MergeGenerator?
+  decreases g, 0
+  {
+    var remains := MapRemove1(g.remains, GenTop(g).key);
+
+    if GenTop(g.top).Next? && GenTop(g.bot).Next?
+        && GenTop(g.top).key == GenTop(g.bot).key then (
+      MergeGenerator(
+        GenPop(g.top),
+        GenPop(g.bot),
+        Next(GenTop(g.top).key,
+            Merge(GenTop(g.top).msg, GenTop(g.bot).msg)),
+        remains)
+    ) else if GenTop(g.top).Next?
+        && (GenTop(g.bot).Next? ==> Keyspace.lt(GenTop(g.top).key, GenTop(g.bot).key)) then (
+      MergeGenerator(
+        GenPop(g.top),
+        g.bot,
+        GenTop(g.top),
+        remains)
+    ) else if GenTop(g.bot).Next? then (
+      MergeGenerator(
+        g.top,
+        GenPop(g.bot),
+        GenTop(g.bot),
+        remains)
+    ) else (
+      MergeGenerator(
+        g.top,
+        g.bot,
+        Done,
+        remains)
+    )
+  }
+
+  lemma lemmaMergeGenPop(g: Generator)
+  requires WF(g)
+  requires GenTop(g).Next?
+  requires g.MergeGenerator?
+  decreases g, 1
+  ensures WF(MergeGenPop(g))
+  {
+    reveal_Lump();
+    var g' := MergeGenPop(g);
+    assert g'.MergeGenerator?;
   }
 
   function {:opaque} GenPop(g: Generator) : (g' : Generator)
@@ -46,10 +184,19 @@ module BucketGenerator {
   requires GenTop(g).Next?
   ensures WF(g')
   ensures g'.remains == MapRemove1(g.remains, GenTop(g).key)
+  decreases g, 2
   {
-    BasicGenerator(
-        g.bucket,
-        IterInc(g.bucket, g.it),
-        MapRemove1(g.remains, GenTop(g).key))
+    reveal_GenTop();
+
+    match g {
+      case BasicGenerator(bucket, it, remains) => (
+        lemmaBasicGenPop(g);
+        BasicGenPop(g)
+      )
+      case MergeGenerator(top, bot, next, remains) => (
+        lemmaMergeGenPop(g);
+        MergeGenPop(g)
+      )
+    }
   }
 }
